verification/tests/DiscountTests.dfy
@@ -33,7 +33,6 @@ module DiscountTests {
   {}
 
   method CalculateOriginalAmountTest()
-    ensures Discount(10, 20, 1000).CalculateOriginalAmount(0) == 0
     ensures Discount(10, 20, 1000).CalculateOriginalAmount(110) == 100
     ensures Discount(10, 20, 1).CalculateOriginalAmount(100) == 99
     ensures Discount(10, 20, 99).CalculateOriginalAmount(100) == 99
